Finished initial_core for ASM and Clight.
Started working on the semantics and simulations.

common/Smallstep.v
@@ -477,9 +477,14 @@ End CLOSURES.
 
 Record semantics : Type := Semantics_gen {
   state: Type;
+  (** A state contains a memory, so we use the following  *)
+  (** setters or getters                                  *)
+  (* If you put them here, you should move the lemmas too *)
+  get_mem: state -> Memory.mem;
+  set_mem: state -> Memory.mem -> state;
   genvtype: Type;
   step : genvtype -> state -> trace -> state -> Prop;
-  initial_state: state -> val -> list val -> Prop;
+  initial_core: state -> val -> list val -> Prop;
   final_state: state -> int -> Prop; (* Make return a val *)
   globalenv: genvtype;
   symbolenv: Senv.t}.
@@ -487,45 +492,44 @@ Record semantics : Type := Semantics_gen {
 (*NEW*)
 Record expressive_semantics : Type :=
   Expressive_Semantics_gen {
-      Sem:> semantics;
-  (** A state contains a memory, so we use the following *)
-  (** setters or getters                                 *)
-  get_mem: state Sem -> Memory.mem;
-  set_mem: state Sem -> Memory.mem -> state Sem;
+      sem:> semantics;
   set_get_mem: forall s,
-      s = set_mem s (get_mem s);
+      s = set_mem sem s (get_mem sem s);
   get_set_mem: forall s m,
-      m = get_mem (set_mem s m);
+      m = get_mem sem (set_mem sem s m);
   (** States before and after external calls are identified *)
   (** external calls are exactly one step                   *)
-  at_external: genvtype Sem ->
-               state Sem ->
+  at_external: genvtype sem ->
+               state sem ->
                option (external_function * list val);
-  after_external: genvtype Sem ->
+  after_external: genvtype sem ->
                   option val ->
-                  state Sem ->
-                  option (state Sem);
+                  state sem ->
+                  option (state sem);
   external_step_lemma:
     forall g s1 ef args t s2,
       at_external g s1 = Some (ef, args) ->
-      step Sem g s1 t s2 ->   
+      step sem g s1 t s2 ->   
       exists vr,
-        external_call ef (symbolenv Sem) args (get_mem s1) t (Val.maketotal vr) (get_mem s2) /\
-        after_external g vr (set_mem s1 (get_mem s2)) = Some s2 
+        external_call ef (symbolenv sem) args (get_mem sem s1) t (Val.maketotal vr) (get_mem sem s2) /\
+        after_external g vr (set_mem sem s1 (get_mem sem s2)) = Some s2 
 }.
 
 (** The form used in earlier CompCert versions, for backward compatibility. *)
-
 Definition Semantics {state funtype vartype: Type}
+                     (get_mem: state -> Memory.mem)
+                     (set_mem: state -> Memory.mem -> state)
                      (step: Genv.t funtype vartype -> state -> trace -> state -> Prop)
-                     (initial_state: state -> Prop)
+                     (initial_core: state -> val -> list val -> Prop)
                      (final_state: state -> int -> Prop)
                      (globalenv: Genv.t funtype vartype)
   :=
   {| state := state;
+     get_mem := get_mem ;
+     set_mem := set_mem ;
      genvtype := Genv.t funtype vartype;
      step := step;
-     initial_state := initial_state;
+     initial_core := initial_core;
      final_state := final_state;
      globalenv := globalenv;
      symbolenv := Genv.to_senv globalenv |}.
@@ -542,15 +546,307 @@ Notation " 'Nostep' L " := (nostep (step L) (globalenv L)) (at level 1) : smalls
 Open Scope smallstep_scope.
 
 (** * Forward simulations between two transition semantics. *)
+ Section ForwardSimulations.
+  
+  Variables L1 L2: semantics.
+  Notation get_mem1:=(get_mem L1).
+  Notation get_mem2:=(get_mem L2).
 
+  (** *Equality Phases*)
+  Section Equality.
+    Record fsim_properties_eq: Type :=
+      {
+        Eqindex: Type;
+        Eqorder: Eqindex -> Eqindex -> Prop;
+        Eqmatch_states: Eqindex -> state L1 -> state L2 -> Prop;  
+        Eqfsim_order_wf: well_founded Eqorder;
+        Eqfsim_match_meminj: forall i s1 s2, Eqmatch_states i s1 s2 ->  (get_mem1 s1) = (get_mem2 s2);
+        (*    fsim_match_initial_states:
+      forall s1 m1 f m2, initial_state L1 (s1,m1) -> Mem.inject f m1 m2 ->
+      exists i, exists s2, initial_state L2 (s2,m2) /\ match_states i f (s1,m1) (s2,m2);*)
+        Eqfsim_match_initial_core:
+          forall s1 fp args, initial_core L1 s1 fp args -> 
+          exists i s2, get_mem1 s1 = get_mem2 s2 /\ initial_core L2 s2 fp args /\ Eqmatch_states i s1 s2;
+        Eqfsim_match_final_states:
+          forall i s1 s2 r ,
+            Eqmatch_states i s1 s2 -> final_state L1 s1 r -> (final_state L2 s2 r);
+        Eqfsim_simulation:
+          forall s1 t s1', Step L1 s1 t s1' ->
+                      forall i s2, Eqmatch_states i s1 s2 ->
+                              exists i', exists s2',
+                                  (Plus L2 s2 t s2' \/ (Star L2 s2 t s2' /\ Eqorder i' i))
+                                  /\ Eqmatch_states i' s1' s2';
+        Eqfsim_public_preserved:
+          forall id, Senv.public_symbol (symbolenv L2) id = Senv.public_symbol (symbolenv L1) id
+      }.
+  
+    
+    Lemma sim_eqSim':
+      forall index order (match_states:index -> state L1 -> state L2 -> Prop),
+      (forall i s1 s2, match_states i s1 s2 ->  (get_mem1 s1) = (get_mem2 s2)) ->
+      fsim_properties L1 L2 index order match_states ->
+      fsim_properties_eq.
+    Proof.
+      intros ? ? ? H HH; inv HH.
+      econstructor; eauto.
+    Qed.
+  End Equality.
+
+  
+  (** *Extension Phases*)
+  Section Extensions.
+    
+   Record fsim_properties_ext: Type :=
+  {
+    Extindex: Type;
+    Extorder: Extindex -> Extindex -> Prop;
+    Extmatch_states: Extindex -> state L1 -> state L2 -> Prop;  
+    Extfsim_order_wf: well_founded Extorder;
+    Extfsim_match_meminj: forall i s1 s2, Extmatch_states i s1 s2 ->  Mem.extends (get_mem1 s1) (get_mem2 s2);
+(*    fsim_match_initial_states:
+      forall s1 m1 f m2, initial_state L1 (s1,m1) -> Mem.inject f m1 m2 ->
+      exists i, exists s2, initial_state L2 (s2,m2) /\ match_states i f (s1,m1) (s2,m2);*)
+    Extfsim_match_initial_states:
+      forall s1, initial_state L1 s1 -> 
+               exists i s2, initial_state L2 s2 /\ Extmatch_states i s1 s2;
+    Extfsim_match_final_states:
+      forall i s1 s2 r ,
+      Extmatch_states i s1 s2 -> final_state L1 s1 r -> (final_state L2 s2 r);
+    Extfsim_simulation:
+      forall s1 t s1', Step L1 s1 t s1' ->
+      forall i s2, Extmatch_states i s1 s2 ->
+      exists i', exists s2',
+         (Plus L2 s2 t s2' \/ (Star L2 s2 t s2' /\ Extorder i' i))
+         /\ Extmatch_states i' s1' s2';
+    Extfsim_public_preserved:
+      forall id, Senv.public_symbol (symbolenv L2) id = Senv.public_symbol (symbolenv L1) id
+  }.
+
+   (** An alternate form of the simulation diagram *)
+   Lemma Extfsim_simulation':
+       forall (SIM:fsim_properties_ext),
+       forall i s1 t s1',
+         Step L1 s1 t s1' ->
+         forall s2, Extmatch_states SIM i s1 s2 ->
+               (exists i', exists s2', Plus L2 s2 t s2' /\
+                                   Extmatch_states SIM i' s1' s2')
+               \/ (exists i', Extorder SIM i' i /\ t = E0 /\ Extmatch_states SIM i' s1' s2).
+   Proof.
+     intros. exploit Extfsim_simulation; eauto.
+     intros [i' [s2' [A B ]]]. intuition.
+     left; exists i'; exists s2'; auto .
+     inv H2. 
+     right; exists i'; eauto.
+     left; exists i'; exists s2'; split; auto. econstructor; eauto.
+   Qed.
+
+   (** *Star version of simulation*)
+    Lemma Extsimulation_star:
+      forall (SIM:fsim_properties_ext),
+      forall s1 t s1', Star L1 s1 t s1' ->
+                  forall i s2,
+                    Extmatch_states SIM  i s1 s2 ->
+                    exists i', exists s2', Star L2 s2 t s2' /\ Extmatch_states SIM  i' s1' s2'.
+    Proof.
+      intros S.
+      induction 1; intros.
+      exists i; exists s2; split; auto. apply star_refl.
+
+      (*split; auto; constructor.
+      apply inject_incr_refl. constructor.*)
+
+      exploit Extfsim_simulation; eauto.
+      intros [i' [s2' [A B]]].
+      exploit IHstar; eauto. intros [i'' [s2'' [E F ]]].
+      exists i'';exists s2''; split; auto. eapply star_trans; eauto.
+      intuition auto. apply plus_star; auto.
+    Qed.
+    
+    (** *Plus version of simulation*)
+    Lemma Extsimulation_plus:
+      forall (SIM: fsim_properties_ext),
+      forall s1 t s1', Plus L1 s1 t s1' ->
+                  forall i s2, Extmatch_states SIM  i s1 s2 -> 
+            (exists i', exists s2', Plus L2 s2 t s2' /\ Extmatch_states SIM  i' s1' s2')
+            \/ (exists i', clos_trans _ (Extorder SIM) i' i /\ t = E0 /\ Extmatch_states SIM  i' s1' s2).
+    Proof.
+      intros S.
+      induction 1 using plus_ind2; intros.
+      (* base case *)
+      exploit Extfsim_simulation'; eauto.
+      intros [[i' [s2' [A B ]]] | [i'  A]].
+      left. exists i', s2'; auto.
+      right; exists i'; intuition.
+      (* inductive case *)
+      exploit Extfsim_simulation'; eauto.
+      intros [[i' [s2' [A B]]] | [i' [A [B C] ]]].
+      exploit Extsimulation_star; eauto. apply plus_star; eauto. eauto.
+      intros [i'' [s2'' [P Q ]]].
+      left; exists i''; exists s2''; split; auto. eapply plus_star_trans; eauto.
+      repeat split; auto.
+      
+      exploit IHplus; eauto.
+      intros [[i'' [s2'' [P Q ]]] | [i'' [P Q]]].
+      subst. simpl. left; exists i''; exists s2''; auto.
+      repeat split; eauto.
+
+      subst. simpl. right; exists i''; intuition auto.
+      eapply t_trans; eauto. eapply t_step; eauto.
+    Qed.
+    
+    Lemma EqEx_sim': 
+        fsim_properties_eq ->
+        fsim_properties_ext.
+    Proof.
+      intros H; inv H.
+      econstructor; eauto.
+      intros.
+      erewrite Eqfsim_match_meminj0; eauto.
+      eapply Mem.extends_refl.
+    Qed.
+
+    Lemma sim_extSim:
+      forall index order (match_states:index -> state L1 -> state L2 -> Prop),
+      (forall i s1 s2, match_states i s1 s2 ->  Mem.extends (get_mem1 s1) (get_mem2 s2)) ->
+      fsim_properties L1 L2 index order match_states ->
+      fsim_properties_ext.
+    Proof.
+      intros ? ? ? H HH; inv HH.
+      econstructor; eauto.
+    Qed.
+
+  End Extensions.
+
+  (** *Injection Phases*)
+  Section Injection.
+    Record fsim_properties_inj: Type :=
+      {  Injindex: Type;
+        Injorder: Injindex -> Injindex -> Prop;
+        Injmatch_states: Injindex -> meminj -> state L1 -> state L2 -> Prop;  
+        Injfsim_order_wf: well_founded Injorder;
+        Injfsim_match_meminj: forall i f s1 s2, Injmatch_states i f s1 s2 ->  Mem.inject f (get_mem1 s1) (get_mem2 s2);
+        Injfsim_match_full: forall i f s1 s2, Injmatch_states i f s1 s2 ->  injection_full f (get_mem1 s1);
+        (*    fsim_match_initial_states:
+      forall s1 m1 f m2, initial_state L1 (s1,m1) -> Mem.inject f m1 m2 ->
+      exists i, exists s2, initial_state L2 (s2,m2) /\ match_states i f (s1,m1) (s2,m2);*)
+        Injfsim_match_initial_states:
+          forall s1, initial_state L1 s1 -> 
+                exists i f s2, initial_state L2 s2 /\ Injmatch_states i f s1 s2;
+        Injfsim_match_final_states:
+          forall i s1 s2 r f,
+            Injmatch_states i f s1 s2 -> final_state L1 s1 r -> (final_state L2 s2 r);
+        Injfsim_simulation:
+          forall s1 t s1' f, Step L1 s1 t s1' ->
+                        forall i s2, Injmatch_states i f s1 s2 ->
+                                exists i', exists s2' f' t',
+                                    (Plus L2 s2 t' s2' \/ (Star L2 s2 t' s2' /\ Injorder i' i))
+                                    /\ Injmatch_states i' f' s1' s2' /\
+                                    Values.inject_incr f f' /\
+                                    inject_trace f' t t';
+        Injfsim_public_preserved:
+          forall id, Senv.public_symbol (symbolenv L2) id = Senv.public_symbol (symbolenv L1) id
+      }.
+
+   (** An alternate form of the simulation diagram *)
+
+    Lemma Injfsim_simulation':
+        forall (SIM:fsim_properties_inj),
+        forall i s1 t s1' f,
+          Step L1 s1 t s1' ->
+          forall s2, Injmatch_states SIM i f s1 s2 ->
+                (exists i', exists s2' f' t',
+                      Plus L2 s2 t' s2' /\
+                      Injmatch_states SIM i' f' s1' s2'
+                      /\ inject_incr f f' /\ inject_trace f' t t')
+                \/ (exists i' f', Injorder SIM i' i /\ t = E0 /\ Injmatch_states SIM i' f' s1' s2
+                  /\ inject_incr f f').
+    Proof.
+      intros. exploit Injfsim_simulation; eauto.
+      intros [i' [s2' [f' [t'[A [B [C D]]]]]]]. intuition.
+      left; exists i'; exists s2'; auto. exists f', t'; eauto.
+      inv H2. inversion D; subst.
+      right; exists i'; eauto.
+      left; exists i'; exists s2',f', (t1 ** t2); split; auto. econstructor; eauto.
+    Qed.
+
+    
+    (** *Star version of simulation*)
+    Lemma Injsimulation_star:
+        forall (SIM:fsim_properties_inj),
+      forall s1 t s1', Star L1 s1 t s1' ->
+                  forall i f s2,
+                    Injmatch_states SIM i f s1 s2 ->
+                    exists i' f', exists s2' t', Star L2 s2 t' s2' /\ Injmatch_states SIM i' f' s1' s2'
+                                       /\ inject_incr f f' /\ inject_trace f' t t'.
+    Proof.
+      intros S.
+      induction 1; intros.
+      exists i, f; exists s2 , nil; split; auto. apply star_refl.
+      split; auto; constructor.
+      apply inject_incr_refl. constructor.
+      exploit Injfsim_simulation; eauto.
+      intros [i' [s2' [f'[t' [A [B [C D]]]]]]].
+      exploit IHstar; eauto. intros [i'' [f'' [s2'' [t'' [E [F [G HH]]]]]]].
+      exists i'';exists f''; exists s2'', (t' ** t''); split; auto. eapply star_trans; eauto.
+      intuition auto. apply plus_star; auto.
+      split; auto. subst t.
+      split; auto.
+      eapply inject_incr_trans; eauto.
+      admit. (*inject trace properties*)
+    Admitted.
+    
+    (** *Plus version of simulation*)
+    Lemma Injsimulation_plus:
+      forall (SIM:fsim_properties_inj),
+      forall s1 t s1', Plus L1 s1 t s1' ->
+                  forall i f s2, Injmatch_states SIM i f s1 s2 -> 
+            (exists i', exists f', exists s2' t', Plus L2 s2 t' s2' /\ Injmatch_states SIM i' f' s1' s2'
+            /\ inject_incr f f' /\ inject_trace f' t t')
+            \/ (exists i', exists f', clos_trans _ (Injorder SIM) i' i /\ t = E0 /\ Injmatch_states SIM i' f' s1' s2
+                           /\ inject_incr f f').
+    Proof.
+      intros S.
+      induction 1 using plus_ind2; intros.
+      (* base case *)
+      exploit Injfsim_simulation'; eauto.
+      intros [[i' [s2' [f' [t' [A [B [C D]]]]]]] | [i' [f' [t' A]]]].
+      left. exists i', f', s2', t'; auto.
+      right; exists i', f' ; intuition.
+      (* inductive case *)
+      exploit Injfsim_simulation'; eauto.
+      intros [[i' [s2' [f' [t' [A [B [C D]]]]]]] | [i' [f' [A [B [C D]]]]]].
+      exploit Injsimulation_star; eauto. apply plus_star; eauto. eauto.
+      intros [i'' [f'' [s2'' [t'' [P [Q [R SS]]]]]]].
+      left; exists i''; exists f''; exists s2'', (t'**t''); split; auto. eapply plus_star_trans; eauto.
+      repeat split; auto.
+      eapply inject_incr_trans; eauto.
+      subst t.
+      admit. (*Some properties about inject_trace*)
+ 
+      
+      exploit IHplus; eauto.
+      intros [[i'' [f'' [s2'' [t' [P [Q [R SS]]]]]]] | [i'' [f'' [P [Q R]]]]].
+      subst. simpl. left; exists i''; exists f''; exists s2'', (t'); auto.
+      repeat split; eauto.
+      eapply inject_incr_trans; eauto.
+      subst. simpl. right; exists i''; exists f''; intuition auto.
+      eapply t_trans; eauto. eapply t_step; eauto.
+      eapply inject_incr_trans; eauto.
+    Admitted.
+    
+  End Injection.
+ End ForwardSimulations.
+ 
 (** The general form of a forward simulation. *)
-
 Record fsim_properties (L1 L2: semantics) (index: Type)
                        (order: index -> index -> Prop)
                        (match_states: index -> state L1 -> state L2 -> Prop) : Prop := {
     fsim_order_wf: well_founded order;
-    fsim_match_initial_states:
+    (*This the old initial states: *)
+    (* fsim_match_initial_states:
       forall s1, initial_state L1 s1 ->
+      exists i, exists s2, initial_state L2 s2 /\ match_states i s1 s2; *)
+    fsim_match_initial_cores:
       exists i, exists s2, initial_state L2 s2 /\ match_states i s1 s2;
     fsim_match_final_states:
       forall i s1 s2 r,
@@ -558,7 +854,7 @@ Record fsim_properties (L1 L2: semantics) (index: Type)
     fsim_simulation:
       forall s1 t s1', Step L1 s1 t s1' ->
       forall i s2, match_states i s1 s2 ->
-      exists i', exists s2',
+      exists i', exists s2', 
          (Plus L2 s2 t s2' \/ (Star L2 s2 t s2' /\ order i' i))
       /\ match_states i' s1' s2';
     fsim_public_preserved:
